Updates

high2/Zeta.High.Verifier.EAC.fst
@@ -4,14 +4,17 @@ open Zeta.Interleave
 open Zeta.App
 open Zeta.Key
 open Zeta.GenKey
+open Zeta.Record
 open Zeta.Time
 open Zeta.MultiSet
 open Zeta.MultiSetHashDomain
 open Zeta.GenericVerifier
 open Zeta.Generic.Blum
 open Zeta.EAC
+open Zeta.High.Verifier
 open Zeta.High.Thread
 open Zeta.High.Interleave
+open Zeta.High.Merkle
 
 module S = FStar.Seq
 module I = Zeta.Interleave
@@ -23,11 +26,15 @@ module GTL=Zeta.Generic.TSLog
 module HI=Zeta.High.Interleave
 module HTL=Zeta.High.TSLog
 
+noeq
 type failure_info (app:app_params) (n:nat) = {
   bi: nat;
   bk: base_key;
   es: eac_state app bk;
-  le: vlog_entry app
+  le: vlog_entry app;
+  lee: ee:vlog_entry_ext app { to_vlog_entry ee = le /\ eac_add ee es = EACFail };
+  vs_pre: v:vtls_t app {v.valid};
+  vs_post: v:vtls_t app {v.valid /\ v == verify_step le vs_pre};
 }
 
 let eac_failure (#app #n:_) (il: neac_log app n)
@@ -35,8 +42,10 @@ let eac_failure (#app #n:_) (il: neac_log app n)
   = let bi = eac_boundary il in
     let bk = eac_fail_key il in
     let es = eac_state_of_key_pre bk il bi in
-    let le = I.index il bi in
-    { bi; bk; es; le}
+    let le = index il bi in
+    let lee = mk_vlog_entry_ext il bi in
+    eac_state_transition bk il bi;
+    { bi; bk; es; le; lee}
 
 let lemma_non_eac_init_addb
   (#app #n:_)
@@ -72,6 +81,36 @@ let lemma_non_eac_init_addb
       not_eq (add_set ep itsl) (evict_set ep itsl) be;
       hash_collision_contra app
     )
+
+let lemma_non_eac_init_addm
+  (#app #n:_)
+  (itsl: neac_log app n
+    {let fi = eac_failure itsl in
+     fi.es = EACInit /\
+     AddM? fi.le})
+  : hash_collision app
+  = let fi = eac_failure itsl in
+    let i = fi.bi in
+    let AddM (gk,v) k k' = index itsl i in
+    let itsli = prefix itsl i in
+    let itsli' = prefix itsl (i+1) in
+    let tid = src itsl i in
+    let vs_pre = cur_thread_state_pre itsl i in
+    let vs_post = cur_thread_state_post itsl i in
+    lemma_cur_thread_state_extend itsl i;
+    assert(vs_post == verify_step (index itsl i) vs_pre);
+
+    assert(eac_add fi.lee fi.es = EACFail);
+    assert(v <> init_value gk || to_base_key gk <> fi.bk);
+
+    lemma_addm_ancestor_is_proving itsli';
+    assert(k' = proving_ancestor itsli k);
+
+    (* k' is in the verifier cache *)
+    //assert(store_contains (thread_store tid ))
+
+
+    admit()
 
 let lemma_neac_implies_hash_collision
   (#app #n:_)
